\documentclass[letterpaper,notitlepage,twoside, fleqn]{article}

% Basic imports, increase margins...
\usepackage[margin=0.75in]{geometry}
% Finite State Machine stuff
\usepackage{pgf}
\usepackage{tikz}
\usetikzlibrary{arrows, automata}
% Format tables nicely
\usepackage[latin1]{inputenc}
\usepackage{array}

\usepackage{amsfonts}
\usepackage{amssymb}
\usepackage{amsmath,amsthm}

\usepackage{algorithm}          %  float wrapper for algorithms.
\usepackage{algpseudocode}      % layout for algorithmicx
\usepackage{float} % http:/ctan.org/pkg/flot - [H] float parameter forces a 'float' (algorithm block) to remain in a location

\renewcommand{\implies}{\Rightarrow} % redefine command "implies"
\renewcommand{\iff}{\Leftrightarrow} % double arrow
\newcommand{\maps}{\rightarrow} % define command "map"
\newcommand{\union}{\cup}
\newcommand{\intersect}{\cap}
\newcommand{\N}{\mathbb{N}} % natural number
\newcommand{\Q}{\mathbb{Q}} % rational number
\newcommand{\R}{\mathbb{R}} % real number
\newcommand{\Z}{\mathbb{Z}} % integers
\newcommand\tab[1][1cm]{\hspace*{#1}} %\tab command

% Add more packages that you use here...

\begin{document}
\title{%
  Homework 7 \\
  \large CS1675 \\
  \large Professor Adriana Kovashka}
\author{Brian Knotten}
\maketitle

\section*{Part I:}
$x = [1 1]$, $y = [0 0]$, $\eta = 0.3$, $\delta_j = z_j (1 - z_j) \Sigma_k W_{kj} \delta_k$ \\
Activation = $\frac{1}{1+e^{-a}}$, $a_j = \Sigma_{i=1}^D w^{(1)}_{ji} x_i + w_{j0}^{(1)}$\\
All weights set to 0.05 \\
\subsection*{Forward Activations:}
$z_1 = \frac{1}{1+e^{-a}}$
\begin{align*}
-a & = x_0 w^{(1)}_{10} + x_1 w^{(1)}_{11} + x_2 w^{(1)}_{12} \\
 & = 1 \cdot 0.05 + 1 \cdot 0.05 + 1 \cdot 0.05 \\
 & = 0.15
 \end{align*}
$z_1 = \frac{1}{1+e^{-0.15}} = 0.5374$ \\\\
$z_2 = \frac{1}{1+e^{-a}}$
\begin{align*}
-a & = x_0 w^{(1)}_{20} + x_1 w^{(1)}_{21} + x_2 w^{(1)}_{22} \\
 & = 1 \cdot 0.05 + 1 \cdot 0.05 + 1 \cdot 0.05 \\
 & = 0.15
 \end{align*}
 $z_2 = \frac{1}{1+e^{-0.15}} = 0.5374$ \\\\
 $y_1 = \frac{1}{1+e^{-a}}$
 \begin{align*}
-a & = z_0 w^{(2)}_{10} + z_1 w^{(2)}_{11} + z_2 w^{(2)}_{12} \\
 & = 1 \cdot 0.05 + 0.5374 \cdot 0.05 + 0.5374 \cdot 0.05 \\
 & = 0.1037
 \end{align*}
  $y_1 = \frac{1}{1+e^{-0.1037}} = 0.5259$ \\\\
  $y_2 = \frac{1}{1+e^{-a}}$
  \begin{align*}
-a & = z_0 w^{(2)}_{20} + z_1 w^{(2)}_{21} + z_2 w^{(2)}_{22} \\
 & = 1 \cdot 0.05 + 0.5374 \cdot 0.05 + 0.5374 \cdot 0.05 \\
 & = 0.1037
 \end{align*}
   $y_2 = \frac{1}{1+e^{-0.1037}} = 0.5259$ 
   \subsection*{Backpropogation:}
   $\delta_k = y_k (1-y_k)(y_k - t_k)$, $t_k$ = desired $y_k$ output = 0, $y_k = y_1 = y_2 = 0.5259$ \\
   $ \frac{\partial E}{\partial w_{kj}^{(2)}} = \delta_k z_j$, $w^{(\tau + 1)} = w^{(\tau)} - \eta \nabla E(w^{(\tau}))$ \\\\
   $\delta_{y1} = 0.5259 \cdot (1 - 0.5259) \cdot (0.5259 - 0) = 0.1311$ \\
   $\delta_{y2} = 0.5259 \cdot (1 - 0.5259) \cdot (0.5259 - 0) = 0.1311$ \\
   $z_0 = 1, z_1 = z_2 = 0.5374, \eta = 0.3, w^{(\tau)} = 0.05$  $\forall w_{kj}$ \\\\
   $w^{(2)}_{10} = w^{(2)}_{10} - 0.3 \cdot \delta_{y1} \cdot z_0 = 0.05 - 0.3 \cdot 0.1311 \cdot 1 = 0.01067$ \\
   $w^{(2)}_{11} = w^{(2)}_{11} - 0.3 \cdot \delta_{y1} \cdot z_1 = 0.05 -0.3 \cdot 0.1311 \cdot 0.5374=0.02886$ \\
   $w^{(2)} _{12} = w^{(2)}_{12} - 0.3 \cdot \delta_{y1} \cdot z_2 = 0.05 -0.3 \cdot 0.1311 \cdot 0.5374=0.02886$\\\\
   $w^{(2)}_{20} = w^{(2)}_{20} - 0.3 \cdot \delta_{y2} \cdot z_0 = 0.05 - 0.3 \cdot 0.1311 \cdot 1 = 0.01067$ \\
   $w^{(2)}_{21} = w^{(2)}_{21} - 0.3 \cdot \delta_{y2} \cdot z_1 = 0.05 -0.3 \cdot 0.1311 \cdot 0.5374=0.02886$ \\
   $w^{(2)}_{22} = w^{(2)}_{22} - 0.3 \cdot \delta_{y2} \cdot z_2 = 0.05 -0.3 \cdot 0.1311 \cdot 0.5374=0.02886$ \\
   \\
   $\delta_j = z_j(1-z_j) \Sigma_k w_{kj} \delta_k$, $z_j = z_j$ from activation $(0.5374)$, $w_{kj} =$ weight from before update (0.05), $\frac{\partial E}{\partial w_{ji}^{(1)}} = \delta_j x_i$
   \begin{align*}
   \delta_{z1} &= z_1 \cdot (1-z_1) \cdot (w^{(2)}_{11} \cdot \delta_{y1} + w^{(2)}_{21} \cdot \delta_{y2})\\
   &= 0.5374 \cdot (1 - 0.5374) \cdot (0.05 \cdot 0.1311 + 0.05 \cdot 0.1311) \\
   &= 0.003259
   \end{align*}
  \begin{align*}
   \delta_{z2} &= z_2 \cdot (1-z_2) \cdot (w^{(2)}_{12} \cdot \delta_{y1} + w^{(2)}_{22} \cdot \delta_{y2})\\
   &= 0.5374 \cdot (1 - 0.5374) \cdot (0.05 \cdot 0.1311 + 0.05 \cdot 0.1311) \\
   &= 0.003259
   \end{align*}
   $w^{(1)}_{10} = w^{(1)}_{10} - 0.3 \cdot \delta_{z1} \cdot x_0 = 0.05 - 0.3 \cdot 0.003259 \cdot 1 = 0.04902$ \\
   $w^{(1)}_{11} = w^{(1)}_{11} - 0.3 \cdot \delta_{z1} \cdot x_1 = 0.05 - 0.3 \cdot 0.003259 \cdot 1 = 0.04902$ \\
   $w^{(1)}_{12} = w^{(1)}_{12} - 0.3 \cdot \delta_{z1} \cdot x_2 = 0.05 - 0.3 \cdot 0.003259 \cdot 1 = 0.04902$ \\\\
   $w^{(1)}_{20} = w^{(1)}_{20} - 0.3 \cdot \delta_{z2} \cdot x_0 = 0.05 - 0.3 \cdot 0.003259 \cdot 1 = 0.04902$ \\
   $w^{(1)}_{21} = w^{(1)}_{21} - 0.3 \cdot \delta_{z2} \cdot x_1 = 0.05 - 0.3 \cdot 0.003259 \cdot 1 = 0.04902$ \\
   $w^{(1)}_{22} = w^{(1)}_{22} - 0.3 \cdot \delta_{z2} \cdot x_2 = 0.05 - 0.3 \cdot 0.003259 \cdot 1 = 0.04902$ \\

   
\end{document}